tla-tree/ImmutableDiskTreeInv.dfy
@@ -4,11 +4,6 @@ module ImmutableDiskTreeInv {
 import opened TreeTypes
 import opened ImmutableDiskTreeImpl
 
-predicate FullView(k:Constants, view:View)
-{
-    forall lba :: 0 <= lba < DiskSize(k) <==> lba in view
-}
-
 predicate SuperblockTypeCorrect(k:Constants, view:View)
     requires PlausibleDiskSize(k)
     requires FullView(k, view)
