tla-tree/MissingLibrary.dfy
@@ -59,4 +59,11 @@ function max(a:int, b:int) : int
     if a>b then a else b
 }
 
+function {:opaque} MemsetSeq<V>(v:V, len:nat) : (s:seq<V>)
+    ensures |s| == len
+    ensures forall i :: 0<=i<len ==> s[i] == v
+{
+    if len == 0 then [] else MemsetSeq(v, len-1) + [v]
+}
+
 } // module
